src/feather_model/basic.lean
@@ -3,47 +3,82 @@ import order.extension.well
 
 universe u
 
+/-!
+In this file, we construct the type of feather terms in our model,
+given the previous level of the model.
+-/
+
 namespace feather_model
 
 open_locale classical
 
-/-- The type of variables in our model. -/
-def V : Type u := ulift ℕ
-
 /--
-A term in our model.
+A term in our model, parametrised by the type of terms in the previous level of the model.
 
 * `var v` is the term representing the variable `v`.
+* `prev e` is a term `e` from the previous level of the model.
+* `univ` represents all of `Type u`.
 * `ty α` is the Lean type `α`.
 * `obj α x` is a Lean object of type `α` and value `x : α`.
 * `apply f x` is the term representing function application of `f` on `x`.
+
+If we are in level `u` of the model, `ty` represents feather objects of type `Type u`, and `obj`
+represents feather objects of type which lies in `Type u`. Notably, `var` is a variable of feather
+objects of type `Type u` or of type which lies in `Type u`. If smaller universes are needed, wrap
+them in `prev`.
+
+Some "error states" representing invalid situations are encoded as `ty pempty`.
 -/
-inductive mterm : Type (u + 1)
-| var : V.{u} → mterm
+inductive mterm (T : Type u) : Type (u + 1)
+| var : V → mterm
+| prev : T → mterm
+| univ : mterm
 | ty : Type u → mterm
 | obj : Π (α : Type u), α → mterm
 | apply : mterm → mterm → mterm
 
+/-- Provides the `has_type` function, which determines if a given term has a given type.
+This is just used for bookkeeping between levels of the model. -/
+class type_data (α : Type*) :=
+(has_type : α → α → Prop)
+(is_type : α → Prop)
+
+variables {T : Type u} [term_struct T]
+
 namespace mterm
 
-def bound : Π (e : mterm), finset V
+def bound : Π (e : mterm T), finset V
 | (var v) := {v}
+| (prev e) := term_struct.bound e
+| univ := ∅
 | (ty α) := ∅
 | (obj α x) := ∅
 | (apply f x) := bound f ∪ bound x
 
 -- A convenient instance to use instead of explicitly calling `bound` all the time.
-instance mterm_has_mem : has_mem V mterm := ⟨λ v e, v ∈ bound e⟩
+instance mterm_has_mem : has_mem V (mterm T) := ⟨λ v e, v ∈ bound e⟩
 
-def subst (v : V) (e : mterm) : Π (f : mterm), mterm
-| (var w) := if v = w then e else var w
-| (ty α) := ty α
-| (obj α x) := obj α x
-| (apply f x) := apply (subst f) (subst x)
+def subst (v : V) : Π (e : mterm T) (f : mterm T), mterm T
+| e (var w) := if v = w then e else var w
+| (prev e) (prev f) := prev (term_struct.subst v e f)
+| _ (prev f) := ty pempty
+| e univ := univ
+| e (ty α) := ty α
+| e (obj α x) := obj α x
+| e (apply f x) := apply (subst e f) (subst e x)
 
-def has_type : Π (e f : mterm), Prop
+def has_type [type_data T] : Π (e f : mterm T), Prop
+| (prev x) (prev α) := type_data.has_type x α
+| (ty α) univ := true
 | (obj α x) (ty β) := α = β
 | _ _ := false
+
+def is_type [type_data T] : Π (e : mterm T), Prop
+| (prev α) := type_data.is_type α
+| (ty α) := true
+| _ := false
+
+instance mterm.type_data [type_data T] : type_data (mterm T) := ⟨has_type, is_type⟩
 
 end mterm
 
@@ -51,48 +86,48 @@ open mterm
 
 section interpretation
 
-/-! Given a context, which here means a  `finset (V × mterm)`, we produce the set of all
+/-! Given a context, which here means a  `finset (V × mterm T)`, we produce the set of all
 *interpretations* of that context: substitutions of Lean objects for these variables
 that satisfy the given context. -/
 
 /--
-We establish a relation on judgments `V × mterm`.
+We establish a relation on judgments `V × mterm T`.
 If `v` occurs bound in a term `f`, then `(v, e)` must precede `(w, f)`.
 
-On a plain context `finset (V × mterm)`, if the transitive closure of this relation forms a
+On a plain context `finset (V × mterm T)`, if the transitive closure of this relation forms a
 strict partial order, we can sort the judgments and provide a set of interpretations for it by
 iteratively substituting along this order.
 -/
-def immediately_precedes (a b : V × mterm) : Prop := a.1 ∈ b.2
+def immediately_precedes (a b : V × mterm T) : Prop := a.1 ∈ b.2
 
 /-- A list of substitutions to perform to yield a interpretation of a collection of variables. -/
-@[reducible] def interpretation := list (V × mterm)
+@[reducible] def interpretation (T : Type u) := list (V × mterm T)
 
 /-- Given an interpretation, evaluate this term. -/
-def interpretation.interpret (I : interpretation) (e : mterm) : mterm :=
-list.foldl (λ (f : mterm) (i : V × mterm), subst i.1 i.2 f) e I
+def interpretation.interpret (I : interpretation T) (e : mterm T) : mterm T :=
+list.foldl (λ (f : mterm T) (i : V × mterm T), subst i.1 i.2 f) e I
 
-/-- A collection of assumptions `V × mterm` is *sortable* if they can be ordered in such a way
+/-- A collection of assumptions `V × mterm T` is *sortable* if they can be ordered in such a way
 where each variable occurs only in substitutions later in the order. -/
-def interpretation.sortable (C : finset (V × mterm)) : Prop :=
+def interpretation.sortable (C : finset (V × mterm T)) : Prop :=
 well_founded (λ a b : C, immediately_precedes a.val b.val)
 
 /-- Assuming a context is sortable, produce a linear order for it. -/
-noncomputable def interpretation.sort_order (C : finset (V × mterm))
+noncomputable def interpretation.sort_order (C : finset (V × mterm T))
   (h : interpretation.sortable C) : linear_order C :=
 well_founded.well_order_extension h
 
 /-- Assuming that a context is sortable, sort it. The precise sort chosen is arbitrary. -/
-noncomputable def interpretation.sort (C : finset (V × mterm)) (h : interpretation.sortable C) :
-  list (V × mterm) :=
+noncomputable def interpretation.sort (C : finset (V × mterm T)) (h : interpretation.sortable C) :
+  list (V × mterm T) :=
 (finset.sort (interpretation.sort_order C h).le C.attach).map subtype.val
 
 /-- Substitutes the term `e` for the variable `v`. If the context contains an assumption `v : α`,
 it is removed. -/
-def interpretation.subst (v : V) (e : mterm) (I : list (V × mterm)) : list (V × mterm) :=
-(I.filter (λ x : V × mterm, x.1 = v)).map (prod.map id (subst v e))
+def interpretation.subst (v : V) (e : mterm T) (I : list (V × mterm T)) : list (V × mterm T) :=
+(I.filter (λ x : V × mterm T, x.1 = v)).map (prod.map id (subst v e))
 
-lemma interpretation.subst_length (v : V) (e : mterm) (I : interpretation) :
+lemma interpretation.subst_length (v : V) (e : mterm T) (I : interpretation T) :
   (interpretation.subst v e I).length ≤ I.length :=
 begin
   unfold interpretation.subst,
@@ -101,11 +136,11 @@ begin
 end
 
 /-- The set of interpretations of a typing judgment `e : type`. -/
-def interpretations (v : V) : Π (type : mterm), set interpretation
+def interpretations (v : V) : Π (type : mterm T), set (interpretation T)
 | (ty α) := ⋃ (x : α), {[⟨v, mterm.obj α x⟩]}
 | _ := ∅
 
-def interpretations' : Π (C : list (V × mterm)), set interpretation
+def interpretations' : Π (C : list (V × mterm T)), set (interpretation T)
 | [] := {[]}
 | (x :: xs) := ⋃ (I ∈ interpretations x.1 x.2),
     have (interpretation.subst x.1 x.2 xs).length < (x :: xs).length,
@@ -113,42 +148,66 @@ def interpretations' : Π (C : list (V × mterm)), set interpretation
     (λ J, I ++ J) '' interpretations' (interpretation.subst x.1 x.2 xs)
 using_well_founded { rel_tac := λ _ _, `[exact ⟨_, measure_wf list.length⟩] }
 
-def plain_context.interpretations (C : plain_context mterm V) : set interpretation :=
-if h : interpretation.sortable C.Γ then interpretations' (interpretation.sort _ h) else ∅
-
-def rir_context.interpretations (C : rir_context mterm V) : set interpretation :=
+def rir_context.interpretations (C : rir_context (mterm T)) : set (interpretation T) :=
 if h : interpretation.sortable (C.Γ ∪ C.Ξ)
 then interpretations' (interpretation.sort _ h) else ∅
 
-def runtime_context.interpretations (C : runtime_context mterm V) : set interpretation :=
+def runtime_context.interpretations (C : runtime_context (mterm T)) : set (interpretation T) :=
 if h : interpretation.sortable (C.Γ ∪ C.Θ.to_finset ∪ C.Ξ)
 then interpretations' (interpretation.sort _ h) else ∅
 
 end interpretation
 
-def runtime_judgments (J : runtime_judgment mterm V) : Prop :=
-∀ (I : interpretation), I ∈ J.ctx.interpretations → (I.interpret J.e).has_type (I.interpret J.type)
+def is_type [type_data T] (C : rir_context (mterm T)) (α : mterm T) : Prop :=
+∀ (I : interpretation T), I ∈ C.interpretations → mterm.is_type (I.interpret α)
 
-def rir_judgments (J : rir_judgment mterm V) : Prop :=
-∀ (I : interpretation), I ∈ J.ctx.interpretations → (I.interpret J.e).has_type (I.interpret J.type)
+inductive runtime_ok [type_data T] : runtime_context (mterm T) → Prop
+| empty : runtime_ok ⟨∅, ∅, ∅⟩
+| Γ (C : runtime_context (mterm T)) (v : V) (α : mterm T) :
+  runtime_ok C → is_type C.rir α → runtime_ok (C + ⟨{(v, α)}, ∅, ∅⟩)
+| Θ (C : runtime_context (mterm T)) (v : V) (α : mterm T) :
+  runtime_ok C → is_type C.rir α → runtime_ok (C + ⟨∅, {(v, α)}, ∅⟩)
+| Ξ (C : runtime_context (mterm T)) (v : V) (α : mterm T) :
+  runtime_ok C → is_type C.rir α → runtime_ok (C + ⟨∅, ∅, {(v, α)}⟩)
 
-def defeq (C : plain_context mterm V) (x y α : mterm) : Prop :=
-∀ (I : interpretation), I ∈ C.interpretations →
+inductive rir_ok [type_data T] : rir_context (mterm T) → Prop
+| empty : rir_ok ⟨∅, ∅⟩
+| Γ (C : rir_context (mterm T)) (v : V) (α : mterm T) :
+  rir_ok C → is_type C α → rir_ok (C ∪ ⟨{(v, α)}, ∅⟩)
+| Ξ (C : rir_context (mterm T)) (v : V) (α : mterm T) :
+  rir_ok C → is_type C α → rir_ok (C ∪ ⟨∅, {(v, α)}⟩)
+
+-- TODO: Add the assertion that we use the relevant resources in `Θ` only once, and that relevant
+-- things are representable.
+structure runtime_judgments [type_data T] (J : runtime_judgment (mterm T)) : Prop :=
+(ok : runtime_ok J.ctx)
+(interpret : ∀ (I : interpretation T), I ∈ J.ctx.interpretations →
+  (I.interpret J.e).has_type (I.interpret J.type))
+
+structure rir_judgments [type_data T] (J : rir_judgment (mterm T)) : Prop :=
+(ok : rir_ok J.ctx)
+(interpret : ∀ (I : interpretation T), I ∈ J.ctx.interpretations →
+  (I.interpret J.e).has_type (I.interpret J.type))
+
+def defeq [type_data T] (C : rir_context (mterm T)) (x y α : mterm T) : Prop :=
+∀ (I : interpretation T), I ∈ C.interpretations →
   I.interpret x = I.interpret y ∧ (I.interpret x).has_type (I.interpret α)
 
-def sort : sort_name → mterm.{u}
+def sort : sort_name → mterm T
 | (sort_name.type n) := ty pempty
 | sort_name.prop := ty (ulift Prop)
 | sort_name.region := ty punit
 
-def representable (C : finset (V × mterm)) (e : mterm) : mterm.{u} :=
+def representable (C : finset (V × mterm T)) (e : mterm T) : mterm T :=
 mterm.obj (ulift Prop) ⟨false⟩
 
-instance : term_struct mterm := {
-  V := V,
+instance [type_data T] : term_struct (mterm T) := {
   var := var,
   bound := bound,
   subst := subst,
+  is_type := is_type,
+  runtime_ok := runtime_ok,
+  rir_ok := rir_ok,
   runtime_judgments := runtime_judgments,
   rir_judgments := rir_judgments,
   defeq := defeq,
