src/feather_model/model.lean
@@ -1,0 +1,39 @@
+import feather_model.basic
+
+open_locale classical
+
+open feather_model
+
+@[reducible] def 𝕋 := mterm (finset V)
+
+/-- To establish a base case for the model, we create the "empty" model level. -/
+instance : term_struct (finset V) := {
+  var := λ v, {v},
+  bound := id,
+  subst := λ v e f, if v ∈ f then f.erase v ∪ e else f,
+  is_type := λ _ _, true,
+  runtime_ok := λ _, true,
+  rir_ok := λ _, true,
+  runtime_judgments := λ _, true,
+  rir_judgments := λ _, true,
+  defeq := λ _ _ _ _, true,
+  sort := λ _, ∅,
+  representable := λ s f, f,
+}
+
+instance : type_data (finset V) := ⟨λ _ _, true, λ _, true⟩
+
+instance : term (finset V) :=
+begin
+  refine_struct { .. };
+  intros; try { trivial },
+  { unfold subst,
+    rw if_neg,
+    assumption, },
+  { unfold subst,
+    rw if_pos,
+    refl,
+    assumption, },
+end
+
+example : term_struct 𝕋 := infer_instance
