src/feather_model/term.lean
@@ -1,0 +1,83 @@
+import feather_model.basic
+
+universe u
+
+open_locale classical
+
+/-!
+In this file, we prove that the model, as defined in `feather_model.basic`,
+produces a lawful type of terms, assuming the same is true for the lower level.
+-/
+
+namespace feather_model
+
+variables {T : Type u} [term_struct T] [type_data T] [term T]
+
+lemma empty_runtime_ok : runtime_ok (⟨∅, ∅, ∅⟩ : runtime_context (mterm T)) :=
+runtime_ok.empty
+
+lemma empty_rir_ok : rir_ok (⟨∅, ∅⟩ : rir_context (mterm T)) :=
+rir_ok.empty
+
+lemma runtime_ok_Γ (C : runtime_context (mterm T)) {v : V} {α : mterm T} :
+  runtime_ok C → is_type C.rir α → runtime_ok (C + ⟨{(v, α)}, ∅, ∅⟩) :=
+runtime_ok.Γ C v α
+
+lemma runtime_ok_Θ (C : runtime_context (mterm T)) {v : V} {α : mterm T} :
+  runtime_ok C → is_type C.rir α → runtime_ok (C + ⟨∅, {(v, α)}, ∅⟩) :=
+runtime_ok.Θ C v α
+
+lemma runtime_ok_Ξ (C : runtime_context (mterm T)) {v : V} {α : mterm T} :
+  runtime_ok C → is_type C.rir α → runtime_ok (C + ⟨∅, ∅, {(v, α)}⟩) :=
+runtime_ok.Ξ C v α
+
+lemma rir_ok_Γ (C : rir_context (mterm T)) {v : V} {α : mterm T} :
+  rir_ok C → is_type C α → rir_ok (C ∪ ⟨{(v, α)}, ∅⟩) :=
+rir_ok.Γ C v α
+
+lemma rir_ok_Ξ (C : rir_context (mterm T)) {v : V} {α : mterm T} :
+  rir_ok C → is_type C α → rir_ok (C ∪ ⟨∅, {(v, α)}⟩) :=
+rir_ok.Ξ C v α
+
+lemma defeq_reflexive (C : rir_context (mterm T)) {x α : mterm T} :
+  C ⊢ x : α → C ⊢ x ≡ x : α :=
+begin
+  intros h I hI,
+  exact ⟨rfl, h.interpret I hI⟩,
+end
+
+lemma defeq_symmetric (C : rir_context (mterm T)) {x y α : mterm T} :
+  C ⊢ x ≡ y : α → C ⊢ y ≡ x : α :=
+begin
+  intros h I hI,
+  obtain ⟨h₁, h₂⟩ := h I hI,
+  rw h₁ at h₂ ⊢,
+  exact ⟨rfl, h₂⟩,
+end
+
+lemma defeq_transitive (C : rir_context (mterm T)) {x y z α : mterm T} :
+  C ⊢ x ≡ y : α → C ⊢ y ≡ z : α → C ⊢ x ≡ z : α :=
+begin
+  intros hxy hyz I hI,
+  obtain ⟨h₁, h₂⟩ := hxy I hI,
+  obtain ⟨h₃, h₄⟩ := hyz I hI,
+  rw [h₁, h₃] at h₂ ⊢,
+  exact ⟨rfl, h₂⟩,
+end
+
+/-
+instance : term (mterm T) := {
+  empty_runtime_ok := empty_runtime_ok,
+  empty_rir_ok := empty_rir_ok,
+  runtime_ok_Γ := runtime_ok_Γ,
+  runtime_ok_Θ := runtime_ok_Θ,
+  runtime_ok_Ξ := runtime_ok_Ξ,
+  rir_ok_Γ := rir_ok_Γ,
+  rir_ok_Ξ := rir_ok_Ξ,
+  defeq_reflexive := defeq_reflexive,
+  defeq_symmetric := defeq_symmetric,
+  defeq_transitive := defeq_transitive,
+}
+-/
+
+end feather_model
